### CMSC424 Class Notes
#### Kaitlyn Yang | February 24, 2021

3. Extraneous Attributes
- attributes that can be safely removed without changing the closure of the rest of the constraints
- &sigma; is extraneous in &alpha; if:
    - if &sigma; is in &alpha;, and
    - F logically implies F' 
    or
    - let y=&alpha;-&sigma;
    - show that y<sup>+</sup> includes &sigma;

Given
F = {A->C, AB->CD} show C is extra in AB->CD
F' = {A->C, AB->D}

- Using Armstrong's:
    - AB->D
    - ABC->CD
    (also)
    - A->C
    - AB -> BC
    (then)
    - AB -> ABC
    - AB -> ABC -> CD
- (AB)<sup>+</sup> = AB = ABC

Given
F = {A->BE, B->C, C->D, AC->DE}, remove extraneous attributes

- For left side of AC->DE:
    - A extraneous? No C<sup>+</sup>=CD, NOT including DE
    - C extraneous? Yes A<sup>+</sup>=ABCDE, incldues DE
-> F = {A->BE, B->C, C->D, A->DE}


Canonical cover for F is a set of dependencies F<sub>c</sub> such that
- F logically implies all dependencies in F<sub>c</sub>
- F<sub>c</sub> logically implies all dependencies in F
- No functional dependency in F<sub>c</sub> contains an extraneous attribute, and all left sides are unique

to do: repeatedly use the union rule to merge right sides, eliminate extraneous attributes until F<sub>c</sub> has no change

ex. 
A->B, A->C, C->D, AC->BD

cover:
A->BC, C->D, AC->BD
- is A extraneous in ac->bd?
    - does (C)<sup>+</sup> have bd? no, C only has cd
- is C extra?
    - a<sup>+</sup> implies abcd

result: A->BC, C->D, A->BD
A->BCD, C->D
final result: A->BC, C->D

Loss-less Decompositions
def. A decomposition of R into (R1, R2) is called lossless if for all legal instance of r(R):
    R1 &cap; R2 -> R1 or R1 &cap; R2 -> R2
in F<sup>+</sup> 

Consider
R=(A,B,C) and F={A->B, B->C}
1. Decompose into R1=(A,B) and R2=(A,C)
2. Is this lossless?
    - Yes: AB &cap; AC = A wich is a key for R1
    - harder to check for B->C as data is in multiple tables
3. on the other hand, R1=(A,B) and R2=(B,C) is good

def
**dependency-preserving decomposition** if
(F<sub>1</sub> &cup; F<sub>2</sub> &cup; F<sub>3</sub> &cup; ... &cup; F<sub>n</sub>)<sup>+</sup> = F<sup>+</sup>

- closure of all carried dependencies must be the same as the original dependencies

### BCNF & How to Achieve It

BCNF:
- recall that given a schema R, and a set of functional dependencies if every FD &alpha; -> &beta; is either
1. trivial
2. &alpha; is a superkey of R

then R is in BCNF without redundancy

**How to decompose into BCNF**

For all dependencies, check if A is a superkey by using attribute closure

if not then
1. choose a dependency in F+ that breaks the BCNF rules, say &alpha; -> &beta;
2. Create R1=&alpha;&beta;
3. Create R2=R-&beta;

ex.
R=(A,B,C)
F={A->B, B->C}
Candidate keys = {A}

*B->C breaks the relation by not being trivial

So:

R1=(B,C)
F1={B->C}
Candidate Keys = {B}
BCNF = true

and

R2 = (A,C)
F2 = {A->B}
Candidate Keys = {A}
BCNF = true

another ex.
R = (A,B,C,D,E)
F = {A->B, BC->D}
Candidate keys = {ACE}
BCNF = Violated by {A->B, BC->D}

so

R1=(A,B)
F1={A->B}
Candidate keys = {A}
BCNF=true

and

R2 = (A,C,D,E)
F2 = {}
Candidate Keys = {ACDE}
BCNF = true